
# Editor.md

![](https://pandao.github.io/editor.md/images/logos/editormd-logo-180x180.png)

![](https://img.shields.io/github/stars/pandao/editor.md.svg) ![](https://img.shields.io/github/forks/pandao/editor.md.svg) ![](https://img.shields.io/github/tag/pandao/editor.md.svg) ![](https://img.shields.io/github/release/pandao/editor.md.svg) ![](https://img.shields.io/github/issues/pandao/editor.md.svg) ![](https://img.shields.io/bower/v/editor.md.svg)

\begin{equation*}
    \sum F_{x}= F(t)-H-F_f = m_1\ddot{x}_1=m_1\ddot{x},\;  \sum F_{y}=0  
\end{equation*}
